PDDL-sema/AST1.thy
@@ -10,33 +10,32 @@ type_synonym pred = name
 type_synonym func = name
 type_synonym pref = name
 
-datatype type = Either (primitives: "name list")
+datatype type = Either (primitives: "name list") | Number
 
 datatype variable = Variable (var_name: name)
 
 datatype object = name: Object (obj_name: name)
 
-datatype symbol = Var variable | Const object
+datatype var_num = Var variable | Num rat 
+datatype var_num_dur = Var variable | Num rat | Duration
+
+datatype symbol = Var variable | Const object | Num rat | Duration
+
+datatype instant_symbol = Var variable | Const object | Num rat
+
+datatype entity = Const object | Num rat
+
+find_theorems name: "Sum*type"
 
 datatype (sym: 'sym) "term" = 
   Sym 'sym
 | Fun func (arguments: "'sym term list") 
 
-datatype (ent: 'ent) f_exp = 
-  NFun func (arguments: "'ent list")
-| Num rat
-| Neg "'ent f_exp"
-| Add "'ent f_exp" "'ent f_exp"
-| Sub "'ent f_exp" "'ent f_exp"
-| Mult "'ent f_exp" "'ent f_exp"
-| Div "'ent f_exp" "'ent f_exp"
-
 datatype (ent: 'ent) atom = 
   Pred (pred: pred) (arguments: "'ent list")
 | Ent_Eq (lhs: 'ent) (rhs: 'ent)
-| Num_Eq "'ent f_exp" "'ent f_exp"
-| Num_Le "'ent f_exp" "'ent f_exp"
-| Num_Lt "'ent f_exp" "'ent f_exp"
+| Num_Le "'ent" "'ent"
+| Num_Lt "'ent" "'ent"
 
 
 datatype ('x, atoms: 'a) GD = 
@@ -72,48 +71,27 @@ datatype upd_op =
 | Increase
 | Decrease
 
-datatype (ent: 'ent) of_upd = OF_Upd func "'ent list" (ret_val: "'ent option")
-datatype ('t, 'exp) nf_upd = NF_Upd upd_op func "'t list" "'exp"
+datatype (ent: 'ent) of_upd = Fun_Upd upd_op func "'ent list" (ret_val: "'ent option")
 
-type_synonym 't s_nf_upd = "('t, 't f_exp) nf_upd"
-
-datatype 'ent simple_update =
-  S_OU "'ent of_upd"
-| S_NU "'ent s_nf_upd"
+datatype 'ent update =
+  S_FU "'ent of_upd"
 | S_Add "'ent atom"
 | S_Del "'ent atom"
 
-datatype ('x, 'ent) simple_effect =
-  Eff "'ent simple_update"
-| Eff_And "('x, 'ent) simple_effect list"
-| Eff_All 'x "('x, 'ent) simple_effect"
-| Eff_When "('x, 'ent atom) GD" "('x, 'ent) simple_effect"
+datatype ('x, 'ent) effect =
+  Eff "'ent update"
+| Eff_And "('x, 'ent) effect list"
+| Eff_All 'x "('x, 'ent) effect"
+| Eff_When "('x, 'ent atom) GD" "('x, 'ent) effect"
 
-datatype 'ent f_exp_da =
-  Duration
-| NFun func (arguments: "'ent list")
-| Num rat
-| Neg "'ent f_exp_da"
-| Add "'ent f_exp_da" "'ent f_exp_da"
-| Sub "'ent f_exp_da" "'ent f_exp_da"
-| Mult "'ent f_exp_da" "'ent f_exp_da"
-| Div "'ent f_exp_da" "'ent f_exp_da"
 
 datatype 'ent f_exp_t = 
   Time
-| MultTime "'ent f_exp"
-
-type_synonym 't d_nf_upd = "('t, 't f_exp_da) nf_upd"
-
-datatype 'ent durative_update =
-  D_Add "'ent atom"
-| D_Del "'ent atom"
-| D_OU "'ent of_upd"
-| D_NU "'ent d_nf_upd"
+| MultTime "'ent term"
 
 datatype 'ent timed_effect = 
-  DUpd_At_Start "'ent durative_update"
-| DUpd_At_End "'ent durative_update"
+  DUpd_At_Start "'ent update"
+| DUpd_At_End "'ent update"
 | DurScaleUp func "'ent list" "'ent f_exp_t"
 | DurScaleDown func "'ent list" "'ent f_exp_t"
 
@@ -127,16 +105,16 @@ datatype ('t) simple_action = Simple_Action
   (name: name)
   (parameters: "(variable \<times> type) list")
   (precondition: "((variable \<times> type) list, 't atom) pre_GD")
-  (effect: "((variable \<times> type) list, 't) simple_effect")
+  (effect: "((variable \<times> type) list, 't) effect")
 
 type_synonym ast_pre_GD = "((variable \<times> type) list, variable term atom) pre_GD"
-type_synonym ast_simple_effect = "((variable \<times> type) list, variable term) simple_effect"
+type_synonym ast_simple_effect = "((variable \<times> type) list, variable term) effect"
 type_synonym ast_simple_action = "variable term simple_action"
 
 datatype 'ent duration_constraint = 
-  DurLe "'ent f_exp"
-| DurGe "'ent f_exp"
-| DurEq "'ent f_exp"
+  DurLe "'ent term"
+| DurGe "'ent term"
+| DurEq "'ent term"
 
 datatype ('t) durative_action = 
   Durative_Action 
@@ -150,20 +128,15 @@ type_synonym ast_da_GD = "((variable \<times> type) list, variable term atom) da
 type_synonym ast_durative_effect = "((variable \<times> type) list, variable term) durative_effect"
 type_synonym ast_durative_action = "variable term durative_action"
 
-datatype ('t) action = 
-  SA "'t simple_action"
-  | DA "'t durative_action"
+datatype ast_action = 
+  SA "var_num term simple_action"
+  | DA "var_num_dur term durative_action"
 
-type_synonym ast_action = "variable term action"
-
-text \<open>A pred declaration contains the pred's name and its
-  argument types.\<close>
 datatype pred_decl = PredDecl
   (predicate: pred)
   (argTs: "type list")
 
 datatype obj_fun_decl = ObjFunDecl (of_name: func) "type list" type
-datatype num_fun_decl = NumFunDecl (nf_name: func) "type list"
 
 datatype derived_pred = 
   DerivedPred pred 
@@ -174,8 +147,7 @@ datatype ast_domain = Domain
   (types: "(name \<times> name) list") \<comment> \<open> \<open>(type, supertype)\<close> declarations. \<close>
   ("consts": "(object \<times> type) list")
   (preds: "pred_decl list")
-  (ofs: "obj_fun_decl list")
-  (nfs: "num_fun_decl list")
+  (funs: "obj_fun_decl list")
   (actions: "ast_action list")
   (derived: "derived_pred list")
 
