PDDL-sema/AST3.thy
@@ -2,4 +2,239 @@ theory AST3
   imports AST2
 begin
   
+type_synonym name = String.literal
+
+type_synonym pred = name
+type_synonym func = name
+type_synonym pref = name
+
+datatype type = Either (primitives: "name list")
+
+datatype variable = Variable (var_name: name)
+
+datatype object = name: Object (obj_name: name)
+
+datatype symbol = Var variable | Const object | Num rat | Duration
+
+datatype (sym: 'sym) "term" = 
+  Sym 'sym
+| Fun func (arguments: "'sym term list") 
+
+datatype (ent: 'ent) f_exp = 
+  NFun func (arguments: "'ent list")
+| Num rat
+| Neg "'ent f_exp"
+| Add "'ent f_exp" "'ent f_exp"
+| Sub "'ent f_exp" "'ent f_exp"
+| Mult "'ent f_exp" "'ent f_exp"
+| Div "'ent f_exp" "'ent f_exp"
+
+datatype (ent: 'ent) atom = 
+  Pred (pred: pred) (arguments: "'ent list")
+| Ent_Eq (lhs: 'ent) (rhs: 'ent)
+| Num_Le "'ent" "'ent"
+| Num_Lt "'ent" "'ent"
+
+
+datatype ('x, atoms: 'a) GD = 
+  Atom 'a
+| Bot
+| Not "('x, 'a) GD"
+| And "('x, 'a) GD" "('x, 'a) GD"
+| Or "('x, 'a) GD" "('x, 'a) GD"
+| Imp "('x, 'a) GD" "('x, 'a) GD"
+| ForAll 'x "('x, 'a) GD"
+| Exists 'x "('x, 'a) GD"
+
+datatype ('x, 'a) pre_GD =
+  PrefGD "pref option" "('x, 'a) GD"
+| ForAll 'x "('x, 'a) pre_GD"
+| And "('x, 'a) pre_GD" "('x, 'a) pre_GD"
+
+
+datatype ('x, atoms: 'a) timed_GD =
+  OverAll "('x, 'a) GD"
+| AtStart "('x, 'a) GD"
+| AtEnd "('x, 'a) GD"
+
+datatype ('x, atoms: 'a) da_GD =
+  ForAll "'x" "('x, 'a) da_GD"
+| And "('x, 'a) da_GD" "('x, 'a) da_GD"
+| PrefTimedGD "pref option" "('x, 'a) timed_GD"
+
+datatype upd_op = 
+  Assign
+| ScaleUp
+| ScaleDown
+| Increase
+| Decrease
+
+datatype (ent: 'ent) of_upd = OF_Upd func "'ent list" (ret_val: "'ent option")
+datatype ('t, 'exp) nf_upd = NF_Upd upd_op func "'t list" "'exp"
+
+type_synonym 't s_nf_upd = "('t, 't f_exp) nf_upd"
+
+datatype 'ent simple_update =
+  S_OU "'ent of_upd"
+| S_NU "'ent s_nf_upd"
+| S_Add "'ent atom"
+| S_Del "'ent atom"
+
+datatype ('x, 'ent) simple_effect =
+  Eff "'ent simple_update"
+| Eff_And "('x, 'ent) simple_effect list"
+| Eff_All 'x "('x, 'ent) simple_effect"
+| Eff_When "('x, 'ent atom) GD" "('x, 'ent) simple_effect"
+
+datatype 'ent f_exp_da =
+  Duration
+| NFun func (arguments: "'ent list")
+| Num rat
+| Neg "'ent f_exp_da"
+| Add "'ent f_exp_da" "'ent f_exp_da"
+| Sub "'ent f_exp_da" "'ent f_exp_da"
+| Mult "'ent f_exp_da" "'ent f_exp_da"
+| Div "'ent f_exp_da" "'ent f_exp_da"
+
+datatype 'ent f_exp_t = 
+  Time
+| MultTime "'ent f_exp"
+
+type_synonym 't d_nf_upd = "('t, 't f_exp_da) nf_upd"
+
+datatype 'ent durative_update =
+  D_Add "'ent atom"
+| D_Del "'ent atom"
+| D_OU "'ent of_upd"
+| D_NU "'ent d_nf_upd"
+
+datatype 'ent timed_effect = 
+  DUpd_At_Start "'ent durative_update"
+| DUpd_At_End "'ent durative_update"
+| DurScaleUp func "'ent list" "'ent f_exp_t"
+| DurScaleDown func "'ent list" "'ent f_exp_t"
+
+datatype ('x, 'ent) durative_effect =
+  Timed_Effect "'ent timed_effect"
+| DEff_And "('x, 'ent) durative_effect" "('x, 'ent) durative_effect" 
+| DEff_All 'x "('x, 'ent) durative_effect"
+| DEff_When "('x, 'ent atom) da_GD" "'ent timed_effect"
+  
+datatype ('t) simple_action = Simple_Action
+  (name: name)
+  (parameters: "(variable \<times> type) list")
+  (precondition: "((variable \<times> type) list, 't atom) pre_GD")
+  (effect: "((variable \<times> type) list, 't) simple_effect")
+
+type_synonym ast_pre_GD = "((variable \<times> type) list, variable term atom) pre_GD"
+type_synonym ast_simple_effect = "((variable \<times> type) list, variable term) simple_effect"
+type_synonym ast_simple_action = "variable term simple_action"
+
+datatype 'ent duration_constraint = 
+  DurLe "'ent f_exp"
+| DurGe "'ent f_exp"
+| DurEq "'ent f_exp"
+
+datatype ('t) durative_action = 
+  Durative_Action 
+    (name: name)
+    (duration: "'t duration_constraint list")
+    (parameters: "(variable \<times> type) list")
+    (condition: "((variable \<times> type) list, 't atom) da_GD")
+    (effect: "((variable \<times> type) list, 't) durative_effect")
+
+type_synonym ast_da_GD = "((variable \<times> type) list, variable term atom) da_GD"
+type_synonym ast_durative_effect = "((variable \<times> type) list, variable term) durative_effect"
+type_synonym ast_durative_action = "variable term durative_action"
+
+datatype ('t) action = 
+  SA "'t simple_action"
+  | DA "'t durative_action"
+
+type_synonym ast_action = "variable term action"
+
+text \<open>A pred declaration contains the pred's name and its
+  argument types.\<close>
+datatype pred_decl = PredDecl
+  (predicate: pred)
+  (argTs: "type list")
+
+datatype obj_fun_decl = ObjFunDecl (of_name: func) "type list" type
+datatype num_fun_decl = NumFunDecl (nf_name: func) "type list"
+
+datatype derived_pred = 
+  DerivedPred pred 
+    (params: "(variable \<times> type) list")
+    ast_pre_GD
+
+datatype ast_domain = Domain 
+  (types: "(name \<times> name) list") \<comment> \<open> \<open>(type, supertype)\<close> declarations. \<close>
+  ("consts": "(object \<times> type) list")
+  (preds: "pred_decl list")
+  (ofs: "obj_fun_decl list")
+  (nfs: "num_fun_decl list")
+  (actions: "ast_action list")
+  (derived: "derived_pred list")
+
+datatype init_asmt = 
+  At rat "object atom"
+  | NotAt rat "object atom"
+  | ObjAsmt func "object list" object
+  | NumAsmt func "object list" rat
+
+
+(* This is used for constraints *)
+datatype ('x, atoms: 'a) ltl_form = 
+  Atom 'a
+| Bot
+| Not "('x, 'a) ltl_form"
+| And "('x, 'a) ltl_form" "('x, 'a) ltl_form"
+| Or "('x, 'a) ltl_form" "('x, 'a) ltl_form"
+| Imp "('x, 'a) ltl_form" "('x, 'a) ltl_form"
+| ForAll "'x" "('x, 'a) ltl_form"
+| AtEnd "('x, 'a) ltl_form"
+| Always "('x, 'a) ltl_form"
+| SometimeAfter "('x, 'a) ltl_form" "('x, 'a) ltl_form"
+| SometimeBefore "('x, 'a) ltl_form" "('x, 'a) ltl_form"
+| AlwaysWithin rat "('x, 'a) ltl_form" "('x, 'a) ltl_form"
+| HoldDuring rat rat "('x, 'a) ltl_form"
+| HoldAfter rat "('x, 'a) ltl_form"
+
+datatype ('x, 'a) pref_con_GD =
+  con_GD "('x, 'a) ltl_form"
+  | ForAll 'x "('x, 'a) pref_con_GD"
+  | And "('x, 'a) pref_con_GD list"
+  | Pref pref "('x, 'a) ltl_form"
+
+type_synonym constraint = "((variable \<times> type) list, symbol term atom) pref_con_GD"
+
+datatype metric_f_exp =
+  Plus "metric_f_exp" "metric_f_exp"
+  | Minus "metric_f_exp" "metric_f_exp"
+  | Times "metric_f_exp" "metric_f_exp"
+  | Divide "metric_f_exp" "metric_f_exp"
+  | Neg "metric_f_exp"
+  | Number rat
+  | FFun func "object list"
+  | IsViolated pref
+
+text \<open>A problem consists of a domain, a list of objects,
+  a description of the initial state, and a description of the goal state.\<close>
+datatype ast_problem = Problem
+  (domain: ast_domain)
+  (init_asmts: "init_asmt list")
+  (objects: "(object \<times> type) list")
+  (goal: "ast_pre_GD")
+  (constraints: "constraint list")
+
+
+subsubsection \<open>Plans\<close>
+type_synonym time = rat
+
+datatype plan_action = 
+  Simple_Plan_Action (name: name) (arguments: "object list")
+| Durative_Plan_Action (name: name) (arguments: "object list") (duration: "time option")
+
+type_synonym plan = "(time \<times> plan_action) list"
+
 end
